tools/Vale/src/emit_common_lemmas.fs
@@ -524,10 +524,16 @@ let build_lemma (env:env) (benv:build_env) (b1:id) (stmts:stmt list) (bstmts:stm
       let ss = build_lemma_ghost_stmts senv stmts in
       [sReveal; sOldS] @ sBlock @ listIf total [sState] @ ss
     else if benv.is_quick then
-      let eFrame = vaApp "state_match" [EVar sM; eFrameExp] in
-      let (_, enss) = collect_specs (List.concat pspecs) in
-      let enss = enss @ [vaApp "state_match" [EVar sM; eFrameExp]] in
-      Emit_common_quick_code.build_proc_body env loc p (EApply (codeName, fArgs)) (and_of_list enss)
+      let range = EVar (Id "range1") in
+      let msg = EString ("***** MODIFIES CLAUSE NOT MET AT " + string_of_loc loc + " *****") in
+      let eFrameX = vaApp "state_match" [EVar sM; eFrameExp] in
+      let eFrameL = EApply (Id "label", [range; msg; eFrameX]) in
+      let (_, enssL) = collect_specs true (List.concat pspecs) in
+      let (_, enssX) = collect_specs false (List.concat pspecs) in
+      let enssL = enssL @ [eFrameL] in
+      let enssX = enssX @ [eFrameX] in
+      let extraEquivs = List.map2 (fun e1 e2 -> EOp (Bop BEquiv, [e1; e2])) enssX enssL in
+      Emit_common_quick_code.build_proc_body env loc p (EApply (codeName, fArgs)) (and_of_list enssL) extraEquivs
     else if benv.is_operand then
       err "operand procedures must be declared extern"
     else
